vera/VerilogToSMT/VerilogToSMT.v
@@ -27,7 +27,8 @@ From vera Require Import Verilog.
 From vera Require Import Common.
 From vera Require EnvStack.
 From vera Require Import Bitvector.
-From vera Require Import SMT.
+From vera Require Import VerilogSMT.
+From vera Require Import SMTQueries.
 Import (coercions) VerilogSMTBijection.
 From vera Require Import Decidable.
 From vera Require Import Tactics.
@@ -202,7 +203,7 @@ Equations mk_bijection (tag : TaggedVariable.Tag) (vars : list (Verilog.variable
     ret (VerilogSMTBijection.insert (tag, var) name__smt tail_bijection prf1 prf2);
   mk_bijection tag [] := ret VerilogSMTBijection.empty.
 
-Definition mk_declarations : list (Verilog.variable * smtname) -> list SMTLib.declaration :=
+Definition mk_declarations : list (Verilog.variable * smtname) -> list SMTQueries.declaration :=
   map (fun '(var, name) => (name, SMTLib.Sort_BitVec (Verilog.varType var))).
 
 Definition all_vars_driven v :=
@@ -219,6 +220,9 @@ Definition verilog_to_smt (name_tag : TaggedVariable.Tag) (var_start : nat) (vmo
     (list_subset (Verilog.module_body_reads (Verilog.modBody vmodule)) (Verilog.module_inputs vmodule))
     "Read from non-module-input"%string ;;
   assert_dec (all_vars_driven vmodule) "Undriven variables"%string ;;
+  assert_dec
+    (list_subset (Verilog.module_body_writes (Verilog.modBody vmodule)) (Verilog.modVariables vmodule))
+    "Unknown variables written to"%string ;;
   let var_assignment := assign_vars var_start (Verilog.modVariables vmodule) in
   nameMap <- mk_bijection name_tag var_assignment ;;
   assertions <- transfer_module_body
@@ -230,12 +234,11 @@ Definition verilog_to_smt (name_tag : TaggedVariable.Tag) (var_start : nat) (vmo
   query_wf <- assert_dec _ "Query not well-formed"%string ;;
   inr {|
       SMT.nameMap := nameMap;
-      SMT.widths := List.map (fun '(var, smtname) => (smtname, Verilog.varType var)) var_assignment;
       SMT.query :=
         {|
-          SMTLib.declarations := mk_declarations var_assignment;
-          SMTLib.assertions := assertions;
-          SMTLib.wf := query_wf;
+          SMTQueries.declarations := mk_declarations var_assignment;
+          SMTQueries.assertions := assertions;
+          SMTQueries.wf := query_wf;
         |};
     |}
 .
