vera/SMTQueries.v
@@ -1,0 +1,443 @@
+From Coq Require Import List.
+From Coq Require Import Logic.FunctionalExtensionality.
+From Coq Require Import Logic.ProofIrrelevance.
+From Coq Require Import BinNums.
+From Coq Require Import ZArith.
+From Coq Require Import Morphisms.
+
+From vera Require Import Tactics.
+From vera Require Import Common.
+
+From SMTCoqApi Require SMTLib.
+
+Import ListNotations.
+
+Fixpoint term_domain (t : SMTLib.term) : list SMTLib.const_sym :=
+  match t with
+  | SMTLib.Term_Const sym => [sym]
+  | SMTLib.Term_Int _ => []
+  | SMTLib.Term_Geq l r => term_domain l ++ term_domain r
+  | SMTLib.Term_Eq l r => term_domain l ++ term_domain r
+  | SMTLib.Term_And l r => term_domain l ++ term_domain r
+  | SMTLib.Term_Or l r => term_domain l ++ term_domain r
+  | SMTLib.Term_Not e => term_domain e
+  | SMTLib.Term_ITE c t f => term_domain c ++ term_domain t ++ term_domain f
+  | SMTLib.Term_True => []
+  | SMTLib.Term_False => []
+  | SMTLib.Term_BVLit _ _ => []
+  | SMTLib.Term_BVConcat l r => term_domain l ++ term_domain r
+  | SMTLib.Term_BVExtract _ _ e => term_domain e
+  | SMTLib.Term_BVUnaryOp _ e => term_domain e
+  | SMTLib.Term_BVBinOp _ l r => term_domain l ++ term_domain r
+  | SMTLib.Term_BVUlt l r => term_domain l ++ term_domain r
+  end
+.
+
+Definition lst_domain (q : list SMTLib.term) : list SMTLib.const_sym :=
+  List.concat (List.map term_domain q).
+
+Definition declaration := (nat * SMTLib.sort)%type.
+
+Record query :=
+  MkQuery
+    {
+      declarations : list declaration;
+      assertions : list SMTLib.term;
+      (* All constants used have been declared *)
+      wf : Forall
+             (fun n => exists s, In (n, s) declarations)
+             (lst_domain assertions)
+    }.
+
+Record decl_term :=
+  MkDeclTerm
+    {
+      dtDeclarations : list declaration;
+      dtTerm : SMTLib.term;
+      (* All constants used have been declared *)
+      dtWf : Forall
+             (fun n => exists s, In (n, s) dtDeclarations)
+             (term_domain dtTerm)
+    }.
+
+Definition domain (q : query) : list SMTLib.const_sym := lst_domain (assertions q).
+
+Definition valuation := nat -> option SMTLib.value.
+
+Definition valuation_set_fun (ρ : valuation) (n : nat) (v : SMTLib.value) : valuation :=
+  fun n' => if n =? n' then Some v else ρ n.
+
+Hint Unfold valuation_set_fun : core.
+
+Definition default_valuation : valuation := fun _ => None.
+
+Inductive value_has_sort : SMTLib.value -> SMTLib.sort -> Prop :=
+| value_has_sort_Bool b : value_has_sort (SMTLib.Value_Bool b) SMTLib.Sort_Bool
+| value_has_sort_Int i : value_has_sort (SMTLib.Value_Int i) SMTLib.Sort_Int
+| value_has_sort_BitVec w bv : value_has_sort (SMTLib.Value_BitVec w bv) (SMTLib.Sort_BitVec w)
+.
+
+Definition valuation_matches_decls (ρ: valuation) (ds: list declaration) : Prop :=
+  Forall (fun '(n, s) => exists v, ρ n = Some v /\ value_has_sort v s) ds.
+
+Definition term_satisfied_by (ρ: valuation) (t: SMTLib.term) : Prop :=
+    SMTLib.interp_term ρ t = Some (SMTLib.Value_Bool true).
+
+Definition decl_term_satisfied_by (ρ: valuation) (t: decl_term) : Prop :=
+  valuation_matches_decls ρ (dtDeclarations t) /\
+    term_satisfied_by ρ (dtTerm t).
+
+Definition satisfied_by (ρ: valuation) (q: query): Prop :=
+  valuation_matches_decls ρ (declarations q) /\
+    Forall (term_satisfied_by ρ) (assertions q).
+
+Lemma decl_term_app_wf t1 t2:
+  Forall (fun n : nat => exists s : SMTLib.sort, In (n, s) (dtDeclarations t1 ++ dtDeclarations t2))
+    (term_domain (dtTerm t1) ++ term_domain (dtTerm t2)).
+Proof.
+  destruct t1, t2. simpl.
+  apply Forall_app.
+  rewrite ! Forall_forall in *.
+  split; intros.
+  - edestruct dtWf0; eauto.
+    eexists. apply List.in_app_iff.
+    eauto.
+  - edestruct dtWf1; eauto.
+    eexists. apply List.in_app_iff.
+    eauto.
+Qed.
+
+Definition not_decl_term (t : decl_term) : decl_term :=
+  {|
+    dtDeclarations := dtDeclarations t;
+    dtTerm := SMTLib.Term_Not (dtTerm t);
+    dtWf := dtWf t
+  |}
+.
+
+Definition and_decl_term (t1 t2 : decl_term) : decl_term :=
+  {|
+    dtDeclarations := dtDeclarations t1 ++ dtDeclarations t2;
+    dtTerm := SMTLib.Term_And (dtTerm t1) (dtTerm t2);
+    dtWf := decl_term_app_wf t1 t2
+  |}
+.
+
+Definition or_decl_term (t1 t2 : decl_term) : decl_term :=
+  {|
+    dtDeclarations := dtDeclarations t1 ++ dtDeclarations t2;
+    dtTerm := SMTLib.Term_Or (dtTerm t1) (dtTerm t2);
+    dtWf := decl_term_app_wf t1 t2
+  |}
+.
+
+Definition term_reflect_if
+  (C : valuation -> Prop)
+  (t: SMTLib.term)
+  (P : valuation -> Prop) : Prop :=
+  forall ρ, C ρ -> term_satisfied_by ρ t <-> P ρ.
+
+Definition term_reflect := term_reflect_if (fun _ => True).
+
+Global Typeclasses Transparent term_reflect.
+
+Global Instance term_reflect_if_proper :
+  Proper
+    (pointwise_relation valuation iff ==> eq ==> pointwise_relation valuation iff ==> iff)
+    term_reflect_if.
+Proof.
+  unfold
+    pointwise_relation,
+    term_reflect_if.
+  repeat intro.
+  setoid_rewrite H.
+  setoid_rewrite H0.
+  setoid_rewrite H1.
+  reflexivity.
+Qed.
+
+Lemma term_reflect_if_elim C t P :
+  term_reflect_if C t P ->
+  (forall ρ, P ρ -> C ρ) ->
+  (forall ρ, term_satisfied_by ρ t -> C ρ) ->
+  term_reflect t P.
+Proof. unfold term_reflect_if. firstorder. Qed.
+
+Lemma term_reflect_if_intro C t P :
+  term_reflect t P ->
+  term_reflect_if C t P.
+Proof. unfold term_reflect_if. firstorder. Qed.
+
+Lemma term_reflect_iff t C P1 P2 :
+  (pointwise_relation _ iff P1 P2) ->
+  term_reflect_if C t P1 ->
+  term_reflect_if C t P2.
+Proof.
+  intros H Hreflect.
+  setoid_rewrite <- H.
+  assumption.
+Qed.
+
+Lemma term_reflect_and q1 q2 P1 P2 :
+  term_reflect q1 P1 ->
+  term_reflect q2 P2 ->
+  term_reflect (SMTLib.Term_And q1 q2) (fun ρ => P1 ρ /\ P2 ρ).
+Proof.
+  unfold term_reflect, term_reflect_if, term_satisfied_by.
+  intros Hrefl1 Hrefl2.
+  simpl.
+  intros ρ _.
+  split; intros * H.
+  - autodestruct_eqn E.
+    Bool.destr_bool.
+    crush.
+  - setoid_rewrite <- Hrefl1 in H; trivial; [].
+    setoid_rewrite <- Hrefl2 in H; trivial; [].
+    destruct H as [H1 H2].
+    rewrite H1, H2.
+    reflexivity.
+Qed.
+
+Lemma term_reflect_or C1 C2 q1 q2 P1 P2 :
+  term_reflect_if C1 q1 P1 ->
+  term_reflect_if C2 q2 P2 ->
+  term_reflect_if
+    (fun ρ =>
+       (exists b, SMTLib.interp_term ρ q1 = Some (SMTLib.Value_Bool b))
+       /\ (exists b, SMTLib.interp_term ρ q2 = Some (SMTLib.Value_Bool b))
+       /\ C1 ρ
+       /\ C2 ρ
+    )
+    (SMTLib.Term_Or q1 q2)
+    (fun ρ => P1 ρ \/ P2 ρ).
+Proof.
+  unfold term_reflect, term_reflect_if, term_satisfied_by.
+  simpl.
+  intros Hrefl1 Hrefl2 ρ [[b1 Hb1] [[b2 Hb2] [HC1 HC2]]].
+  specialize (Hrefl1 ρ ltac:(trivial)).
+  specialize (Hrefl2 ρ ltac:(trivial)).
+  rewrite Hb1, Hb2 in *. clear Hb1 Hb2.
+  split; intros * H.
+  - inv H.
+    Bool.destr_bool; crush.
+  - setoid_rewrite <- Hrefl1 in H; trivial; [].
+    setoid_rewrite <- Hrefl2 in H; trivial; [].
+    destruct H as [H|H];
+      inv H;
+      Bool.destr_bool.
+Qed.
+
+Definition satisfiable (q: query) : Prop :=
+  exists ρ, satisfied_by ρ q.
+
+Definition unsatisfiable (q: query) : Prop :=
+  forall ρ, ~ satisfied_by ρ q.
+
+Definition valid (q: query) : Prop :=
+  forall ρ, satisfied_by ρ q.
+
+Definition invalid (q: query) : Prop :=
+  exists ρ, ~ satisfied_by ρ q.
+
+Lemma valid_satisfiable q :
+  valid q -> satisfiable q.
+Proof.
+  unfold valid, satisfiable.
+  intros.
+  exists default_valuation.
+  auto.
+Qed.
+
+Lemma unsatisfiable_invalid q :
+  unsatisfiable q -> invalid q.
+Proof.
+  unfold valid, satisfiable.
+  intros.
+  exists default_valuation.
+  auto.
+Qed.
+
+Infix "⊧" := satisfied_by (at level 20).
+
+Definition smt_reflect_if (C: valuation -> Prop) (q: query) (P : valuation -> Prop): Prop :=
+  forall ρ, C ρ -> ρ ⊧ q <-> P ρ.
+
+Definition smt_reflect := smt_reflect_if (fun _ => True).
+
+Global Instance smt_reflect_if_proper :
+  Proper
+    (pointwise_relation valuation iff ==> eq ==> pointwise_relation valuation iff ==> iff)
+    smt_reflect_if.
+Proof.
+  unfold
+    pointwise_relation,
+    smt_reflect_if.
+  repeat intro.
+  setoid_rewrite H.
+  setoid_rewrite H0.
+  setoid_rewrite H1.
+  reflexivity.
+Qed.
+
+Global Instance smt_reflect_proper :
+  Proper
+    (eq ==> pointwise_relation valuation iff ==> iff)
+    smt_reflect.
+Proof. unfold smt_reflect. typeclasses eauto. Qed.
+
+Lemma smt_reflect_if_elim C t P :
+  smt_reflect_if C t P ->
+  (forall ρ, P ρ -> C ρ) ->
+  (forall ρ, satisfied_by ρ t -> C ρ) ->
+  smt_reflect t P.
+Proof. unfold smt_reflect_if. firstorder. Qed.
+
+Lemma smt_reflect_if_intro C t P :
+  smt_reflect t P ->
+  smt_reflect_if C t P.
+Proof. unfold smt_reflect_if. firstorder. Qed.
+
+Lemma combine_wf q1 q2 :
+  List.Forall
+    (fun n : nat => exists s : SMTLib.sort, List.In (n, s) (declarations q1 ++ declarations q2))
+    (lst_domain (assertions q1 ++ assertions q2)).
+Proof.
+  destruct q1, q2.
+  unfold lst_domain in *.
+  rewrite ! List.Forall_forall in *.
+  simpl in *.
+  rewrite List.Forall_forall in *.
+  intros n H.
+  rewrite
+    <- List.flat_map_concat_map,
+    List.flat_map_app,
+    List.in_app_iff
+    in *.
+  setoid_rewrite List.in_app_iff.
+  destruct H.
+  - edestruct wf0 as [n' Hwf]; eauto.
+  - edestruct wf1 as [n' Hwf]; eauto.
+Qed.
+
+Definition combine (q1 q2: query) : query :=
+  {|
+    declarations := declarations q1 ++ declarations q2;
+    assertions := assertions q1 ++ assertions q2;
+    wf := combine_wf q1 q2
+  |}.
+
+Lemma concat_conj :
+  forall q1 q2 P1 P2,
+    smt_reflect q1 P1 ->
+    smt_reflect q2 P2 ->
+    smt_reflect (combine q1 q2) (fun ρ => P1 ρ /\ P2 ρ).
+Proof.
+  destruct q1, q2.
+  unfold smt_reflect, smt_reflect_if, satisfied_by, combine.
+  simpl.
+  intros.
+  setoid_rewrite List.Forall_app.
+  firstorder.
+Qed.
+
+Lemma lst_domain_app xs ys :
+  lst_domain (xs ++ ys) = lst_domain xs ++ lst_domain ys.
+Proof.
+  unfold lst_domain.
+  now rewrite List.map_app, List.concat_app.
+Qed.
+
+Lemma lst_domain_cons x xs :
+  lst_domain (x :: xs) = term_domain x ++ lst_domain xs.
+Proof. reflexivity. Qed.
+
+Program Definition add_assertion
+  (a : SMTLib.term)
+  (q : query)
+  (domain_wf : list_subset (term_domain a) (domain q))
+  : query :=
+  {|
+    assertions := a :: assertions q;
+    declarations := declarations q
+  |}.
+Next Obligation.
+  simpl.
+  rewrite lst_domain_cons.
+  unfold list_subset in domain_wf.
+  rewrite List.Forall_app in *.
+  destruct q. cbn in *.
+  rewrite ! List.Forall_forall in *.
+  firstorder.
+Qed.
+
+Lemma add_assertion_reflect_if :
+  forall t q C P1 P2 domain_wf,
+    term_reflect_if C t P1 ->
+    smt_reflect_if C q P2 ->
+    smt_reflect_if C (add_assertion t q domain_wf) (fun ρ => P1 ρ /\ P2 ρ).
+Proof.
+  destruct q.
+  unfold smt_reflect, smt_reflect_if, term_reflect, satisfied_by, combine.
+  simpl.
+  intros.
+  setoid_rewrite List.Forall_cons_iff.
+  firstorder.
+Qed.
+
+Lemma add_assertion_reflect :
+  forall t q P1 P2 domain_wf,
+    term_reflect t P1 ->
+    smt_reflect q P2 ->
+    smt_reflect (add_assertion t q domain_wf) (fun ρ => P1 ρ /\ P2 ρ).
+Proof. intros. apply add_assertion_reflect_if; eassumption. Qed.
+
+Lemma unsat_smt_reflect_false q :
+  unsatisfiable q <-> smt_reflect q (fun _ => False).
+Proof.
+  unfold smt_reflect, satisfied_by, combine.
+  simpl.
+  intros.
+  firstorder.
+Qed.
+
+Lemma smt_reflect_if_rewrite : forall C P2 P1 q,
+    (forall ρ, C ρ -> P1 ρ <-> P2 ρ) ->
+    (smt_reflect_if C q P1 <-> smt_reflect_if C q P2).
+Proof.
+  unfold smt_reflect, smt_reflect_if.
+  intros * HP.
+  split; intros.
+  - rewrite <- HP; eauto.
+  - rewrite HP; eauto.
+Qed.
+
+Lemma smt_reflect_rewrite : forall P2 P1 q,
+    (forall ρ, P1 ρ <-> P2 ρ) ->
+    (smt_reflect q P1 <-> smt_reflect q P2).
+Proof. intros. eapply smt_reflect_if_rewrite. eauto. Qed.
+
+Lemma unsat_negation q P :
+  smt_reflect q P ->
+  unsatisfiable q ->
+  (forall ρ, ~ P ρ).
+Proof.
+  unfold smt_reflect, smt_reflect_if, unsatisfiable.
+  intros Hreflect Hunsat * contra.
+  repeat match goal with
+         | [ H : forall (_ : valuation), _ |- _ ] => specialize (H ρ)
+         end.
+  apply Hreflect in contra; trivial.
+  contradiction.
+Qed.
+
+Lemma incompatible_reflect q1 q2 P1 P2 :
+  smt_reflect q1 P1 ->
+  smt_reflect q2 P2 ->
+  (forall ρ, ~ satisfied_by ρ (combine q1 q2)) ->
+  (forall ρ, ~ (P1 ρ /\ P2 ρ)).
+Proof.
+  intros Hq1P1 Hq2P2 Hunsat.
+  eapply unsat_negation.
+  - eauto using concat_conj.
+  - eauto.
+Qed.
